Coq/safe.v
@@ -4,12 +4,1390 @@ Require Import loo_properties.
 Require Import loo_reduction_properties.
 Require Import decoupled_classical_properties.
 Require Import decoupling.
+Require Import sbst_decoupled.
 Require Import function_operations.
 Require Import List.
 Require Import CpdtTactics.
 Require Import Coq.Logic.FunctionalExtensionality.
 
-Print reduction.
+Lemma substmt_trans :
+  forall s2 s3, substmt s2 s3 ->
+           forall s1, substmt s1 s2 ->
+                 substmt s1 s3.
+Proof.
+  intros s2 s3 Hsub;
+    induction Hsub;
+    intros;
+    auto.
+
+  - apply sub_if1;
+      eauto.
+
+  - apply sub_if2;
+      eauto.
+
+  - apply sub_stmt1;
+      eauto.
+
+  - apply sub_stmt2;
+      eauto.
+
+Qed.
+
+Hint Resolve substmt_trans : loo_db.
+
+Lemma reduction_field_change :
+  forall M σ1 σ2, M ∙ σ1 ⤳ σ2 ->
+             forall χ1 ϕ1 ψ1 χ2 ϕ2 ψ2,
+               σ1 = (χ1, ϕ1 :: ψ1) ->
+               σ2 = (χ2, ϕ2 :: ψ2) ->
+               forall α o1 o2 f v1 v2,
+                 mapp σ1 α = Some o1 ->
+                 mapp σ2 α = Some o2 ->
+                 flds o1 f = Some v1 ->
+                 flds o2 f = Some v2 ->
+                 v1 <> v2 ->
+                 exists x y s C, contn ϕ1 = c_stmt ((x ◌ f) ≔ (r_ y) ;; s) /\
+                            ⌊ x ⌋ σ1 ≜ (v_addr α) /\
+                            classOf this σ1 C /\
+                            classOf x σ1 C /\
+                            ⌊ y ⌋ σ1 ≜ v2.
+Proof.
+  intros M σ1 σ2 Hred;
+    induction Hred;
+    intros;
+    try solve [repeat simpl_crush;
+               repeat map_rewrite;
+               simpl in *;
+               crush].
+
+  - subst; repeat simpl_crush.
+    destruct (eq_dec α α0);
+      subst.
+    + destruct (eq_dec f0 f);
+        subst;
+        eauto.
+      * exists y, x, s, C;
+          repeat split;
+          eauto.
+        repeat map_rewrite.
+        rewrite H5 in H13;
+          inversion H13;
+          subst.
+        assert (Htmp : o2 =
+                       {|
+                         cname := cname o1;
+                         flds := fun x : fld => if eqb x f then Some v else flds o1 x;
+                         meths := meths o1 |});
+          [crush|rewrite Htmp in H16; unfold flds in *].
+        assert (Hflds : (let (_, flds, _) := o1 in flds) = (flds o1));
+          [auto|rewrite Hflds in H16].
+        eq_auto.
+        crush.
+
+      * repeat map_rewrite.
+        rewrite H5 in H13;
+          inversion H13;
+          subst.
+        assert (Htmp : o2 =
+                       {|
+                         cname := cname o1;
+                         flds := fun x : fld => if eqb x f then Some v else flds o1 x;
+                         meths := meths o1 |});
+          [crush|rewrite Htmp in H16; unfold flds in *].
+        assert (Hflds : (let (_, flds, _) := o1 in flds) = (flds o1));
+          [auto|rewrite Hflds in H16].
+        eq_auto.
+        crush.
+    + repeat map_rewrite.
+      crush.
+
+  - subst; repeat simpl_crush.
+    destruct (eq_dec α α0);
+      subst.
+    + eapply fresh_heap_some_contradiction; eauto.
+    + repeat map_rewrite.
+      crush.
+
+Qed.
+
+Lemma reductions_prop_change :
+  forall M σ1 σ2, reductions M σ1 σ2 ->
+             forall P, ~ P σ1 ->
+                  P σ2 ->
+                  exists σ σ', M ∙ σ ⤳ σ' /\
+                          ~ P σ /\
+                          P σ' /\
+                          (reductions M σ1 σ \/ σ1 = σ) /\
+                          (reductions M σ' σ2 \/ σ2 = σ').
+Proof.
+  intros M σ1 σ2 Hred;
+    induction Hred;
+    intros;
+    eauto.
+
+  - repeat eexists;
+      eauto.
+
+  - destruct (excluded_middle (P σ2)) as [Hprop|Hprop].
+    + destruct (IHHred P); auto;
+        destruct_exists_loo;
+        andDestruct.
+      match goal with
+      | [Ha : reductions ?M ?σ1 ?σ \/ ?σ1 = ?σ,
+              Hb : reductions ?M ?σ' ?σ2 \/ ?σ2 = ?σ' |- _] =>
+       destruct Ha, Hb
+      end;
+        subst;
+        try solve [repeat eexists; eauto with loo_db].
+    + repeat eexists; eauto.
+
+Qed.
+
+Check reduction_field_change.
+
+
+Inductive stmt_in_method : mdl -> heap -> addr -> mth -> stmt -> Prop :=
+| in_mth : forall χ α m o M C CDef zs sm s, χ α = Some o ->
+                                       cname o = C ->
+                                       M C = Some CDef ->
+                                       c_meths CDef m = Some (zs, sm) ->
+                                       substmt s sm ->
+                                       stmt_in_method M χ α m s.
+
+Inductive method_is_called : config -> addr -> mth -> partial_map var value -> Prop :=
+| meth_called : forall x y m β s α ϕ χ ψ, contn ϕ = c_stmt (s_meth x y m β ;; s) ->
+                                     ⌊ y ⌋ (χ, ϕ :: ψ) ≜ (v_addr α) ->
+                                     method_is_called (χ, ϕ::ψ) α m (β ∘ (vMap ϕ)).
+
+Hint Constructors method_is_called stmt_in_method : loo_db.
+
+Lemma arising_frame_is_method_call_reduction :
+  forall M σ1 σ2, M ∙ σ1 ⤳ σ2 ->
+             forall χ1 χ2 ϕ1 ϕ2 ψ1 ψ2,
+               σ1 = (χ1, ϕ1 :: ψ1) ->
+               σ2 = (χ2, ϕ2 :: ψ2) ->
+               length (snd σ1) < length (snd σ2) ->
+               (exists α m β s, method_is_called σ1 α m β /\
+                           contn ϕ2 = c_stmt s /\
+                           stmt_in_method M χ1 α m s).
+Proof.
+  intros M σ1 σ2 Hred;
+    induction Hred;
+    intros;
+    subst;
+    crush;
+    repeat simpl_crush.
+
+  exists α, m, (ps ∘ vMap ϕ1), s;
+    repeat split;
+    simpl in *;
+    eauto with loo_db.
+  eapply meth_called; eauto.
+
+Qed.
+
+(*Lemma arising_frame_is_method_call_reduction' :
+  forall M σ1 σ2, M ∙ σ1 ⤳ σ2 ->
+             forall χ1 χ2 ψ1 ψ2,
+               σ1 = (χ1, ψ1) ->
+               σ2 = (χ2, ψ2) ->
+               (forall ϕ1, In ϕ1 ψ1 ->
+                      (exists ψ', ψ1 = ψ' ++ ϕ1 :: nil) \/
+                      (exists α m β s, method_is_called σ1 α m β /\
+                                  contn ϕ2 = c_stmt s /\
+                                  stmt_in_method M χ1 α m s) \/
+                      (exists χ ϕ ψ α m β s, reductions M σ1 (χ, ϕ :: ψ) /\
+                                        reductions M (χ, ϕ :: ψ) σ2 /\
+                                        method_is_called (χ, ϕ :: ψ) α m β /\
+                                        (contn ϕ2 = c_stmt s \/ exists x, contn ϕ2 = c_hole x s) /\
+                                        stmt_in_method M χ α m s)) ->
+               forall ϕ2, In ϕ2 ψ2 ->
+                     (exists ψ', ψ2 = ψ' ++ ϕ2 :: nil) \/
+                     (exists α m β s, method_is_called σ1 α m β /\
+                                 contn ϕ2 = c_stmt s /\
+                                 stmt_in_method M χ1 α m s) \/
+                     (exists χ ϕ ψ α m β s, reductions M σ1 (χ, ϕ :: ψ) /\
+                                       reductions M (χ, ϕ :: ψ) σ2 /\
+                                       method_is_called (χ, ϕ :: ψ) α m β /\
+                                       (contn ϕ2 = c_stmt s \/ exists x, contn ϕ2 = c_hole x s) /\
+                                       stmt_in_method M χ α m s).
+Proof.
+  intros M σ1 σ2 Hred;
+    induction Hred;
+    intros;
+    subst;
+    repeat simpl_crush.
+
+  - admit.
+
+Qed.*)
+
+Lemma arising_frame_is_method_call_reductions :
+  forall M σ1 σ2, reductions M σ1 σ2 ->
+             forall χ1 χ2 ϕ1 ψ2,
+               σ1 = (χ1, ϕ1 :: nil) ->
+               σ2 = (χ2, ψ2) ->
+               forall ϕ2, In ϕ2 ψ2 ->
+                     (exists ψ', ψ2 = ψ' ++ ϕ2 :: nil) \/
+                     (exists α m β s, method_is_called σ1 α m β /\
+                                 contn ϕ2 = c_stmt s /\
+                                 stmt_in_method M χ1 α m s) \/
+                     (exists χ ϕ ψ α m β s, reductions M σ1 (χ, ϕ :: ψ) /\
+                                       reductions M (χ, ϕ :: ψ) σ2 /\
+                                       method_is_called (χ, ϕ :: ψ) α m β /\
+                                       (contn ϕ2 = c_stmt s \/ exists x, contn ϕ2 = c_hole x s) /\
+                                       stmt_in_method M χ α m s).
+Proof.
+  intros M σ1 σ2 Hred;
+    induction Hred;
+    intros;
+    subst.
+
+  - inversion H;
+      subst;
+      repeat simpl_crush;
+      try solve [left;
+                 match goal with
+                 | [H : In ?ϕ (?ϕ' :: nil)|- _] =>
+                   inversion H;
+                   subst; [|crush]
+                 end;
+                 match goal with
+                 | [|- exists ψ', ?ϕ2 :: nil = ψ' ++ ?ϕ2 :: nil ] =>
+                   exists nil;
+                   simpl;
+                   eauto
+                 end].
+
+    + inversion H2;
+        subst;
+        [right; left|left].
+      * repeat eexists;
+          eauto; [|crush].
+        inversion H6;
+          subst;
+          simpl in *;
+          simpl_crush;
+          eauto.
+      * inversion H0; subst;
+          [|crush].
+        match goal with
+        | [|- exists ψ', ?ϕ1 :: ?ϕ2 :: nil = ψ' ++ ?ϕ2 :: nil ] =>
+          exists (ϕ1 :: nil);
+            simpl;
+            eauto
+        end.
+
+  - admit.
+Admitted.
+               
+
+(*Lemma arising_frame_is_method_call_reductions :
+  forall M σ1 σ2, reductions M σ1 σ2 ->
+             forall χ1 χ2 ϕ1 ϕ2 ψ1 ψ2,
+               σ1 = (χ1, ϕ1 :: ψ1) ->
+               σ2 = (χ2, ϕ2 :: ψ2) ->
+               length (snd σ1) < length (snd σ2) ->
+               (exists α m β s, method_is_called σ1 α m β /\
+                           contn ϕ2 = c_stmt s /\
+                           stmt_in_method M χ1 α m s) \/
+               (exists χ ϕ ψ α m β s, reductions M σ1 (χ, ϕ :: ψ) /\
+                                 method_is_called (χ, ϕ :: ψ) α m β /\
+                                 contn ϕ2 = c_stmt s /\
+                                 stmt_in_method M χ α m s).
+Proof.
+  intros M σ1 σ2 Hred;
+    induction Hred;
+    intros;
+    subst;
+    repeat simpl_crush;
+    simpl in *.
+
+  - left; eapply arising_frame_is_method_call_reduction; simpl; eauto.
+
+  - inversion H; subst;
+      repeat simpl_crush.
+    + simpl in *.
+      right.
+      repeat eexists; eauto with loo_db.
+      inversion H7;
+        subst;
+        simpl in *;
+        simpl_crush;
+        auto.
+
+    + simpl in *.
+      destruct (IHHred χ1 χ2 ϕ1 ϕ ψ1 ψ2) as [Ha|Ha];
+        auto.
+      * left; auto.
+        repeat destruct_exists_loo;
+          andDestruct.
+        exists α, m, β, s;
+          repeat split;
+          auto.
+        inversion Hb0;
+          subst.
+        eapply in_mth; eauto.
+        eapply substmt_trans;
+          eauto.
+        rewrite Ha0 in H7;
+          inversion H7;
+          subst;
+          crush.
+
+      * right.
+        repeat destruct_exists_loo;
+          andDestruct.
+        exists χ, ϕ0, ψ, α, m, β, s;
+          repeat split;
+          auto.
+        inversion Hb; subst.
+        eapply in_mth; eauto.
+        eapply substmt_trans;
+          eauto.
+        rewrite Ha1 in H7;
+          inversion H7;
+          subst;
+          crush.
+
+    + simpl in *.
+      destruct (IHHred χ1 χ2 ϕ1 ϕ ψ1 ψ2) as [Ha|Ha];
+        auto.
+      * left; auto.
+        repeat destruct_exists_loo;
+          andDestruct.
+        exists α0, m, β, s;
+          repeat split;
+          auto.
+        inversion Hb0;
+          subst.
+        eapply in_mth; eauto.
+        eapply substmt_trans;
+          eauto.
+        rewrite Ha0 in H6;
+          inversion H6;
+          subst;
+          crush.
+
+      * right.
+        repeat destruct_exists_loo;
+          andDestruct.
+        exists χ, ϕ0, ψ, α0, m, β, s;
+          repeat split;
+          auto.
+        inversion Hb; subst.
+        eapply in_mth; eauto.
+        crush.
+        eapply substmt_trans;
+          eauto.
+        rewrite Ha1 in H6;
+          inversion H6;
+          subst;
+          crush.
+
+    + simpl in *.
+      destruct (IHHred χ1 χ ϕ1 ϕ ψ1 ψ) as [Ha|Ha];
+        auto.
+      * left; auto.
+        repeat destruct_exists_loo;
+          andDestruct.
+        exists α0, m, β, s;
+          repeat split;
+          auto.
+        inversion Hb0;
+          subst.
+        eapply in_mth; eauto.
+        eapply substmt_trans;
+          eauto.
+        rewrite Ha0 in H1;
+          inversion H1;
+          subst;
+          crush.
+
+      * right.
+        repeat destruct_exists_loo;
+          andDestruct.
+        exists χ0, ϕ0, ψ0, α0, m, β, s;
+          repeat split;
+          auto.
+        inversion Hb; subst.
+        eapply in_mth; eauto.
+        eapply substmt_trans;
+          eauto.
+        rewrite Ha1 in H1;
+          inversion H1;
+          subst;
+          crush.
+
+    + simpl in *.
+      destruct (IHHred χ1 χ ϕ1 ϕ ψ1 ψ) as [Ha|Ha];
+        auto.
+      * left; auto.
+        repeat destruct_exists_loo;
+          andDestruct.
+        exists α0, m, β, s;
+          repeat split;
+          auto.
+        inversion Hb0;
+          subst.
+        eapply in_mth; eauto.
+        eapply substmt_trans;
+          eauto.
+        rewrite Ha0 in H3;
+          inversion H3;
+          subst;
+          crush.
+
+      * right.
+        repeat destruct_exists_loo;
+          andDestruct.
+        exists χ0, ϕ0, ψ0, α0, m, β, s;
+          repeat split;
+          auto.
+        inversion Hb; subst.
+        eapply in_mth; eauto.
+        eapply substmt_trans;
+          eauto.
+        rewrite Ha1 in H3;
+          inversion H3;
+          subst;
+          crush.
+
+    + simpl in *.
+      destruct (IHHred χ1 χ2 ϕ1 ϕ ψ1 ψ2) as [Ha|Ha];
+        auto.
+      * left; auto.
+        repeat destruct_exists_loo;
+          andDestruct.
+        exists α, m, β, s1;
+          repeat split;
+          auto.
+        inversion Hb0;
+          subst.
+        eapply in_mth; eauto.
+        eapply substmt_trans;
+          eauto.
+        rewrite Ha0 in H5;
+          inversion H5;
+          subst;
+          crush.
+
+      * right.
+        repeat destruct_exists_loo;
+          andDestruct.
+        exists χ, ϕ0, ψ, α, m, β, s1;
+          repeat split;
+          auto.
+        inversion Hb; subst.
+        eapply in_mth; eauto.
+        eapply substmt_trans;
+          eauto.
+        rewrite Ha1 in H5;
+          inversion H5;
+          subst;
+          crush.
+
+    + simpl in *.
+      destruct (IHHred χ1 χ2 ϕ1 ϕ ψ1 ψ2) as [Ha|Ha];
+        auto.
+      * left; auto.
+        repeat destruct_exists_loo;
+          andDestruct.
+        exists α, m, β, s2;
+          repeat split;
+          auto.
+        inversion Hb0;
+          subst.
+        eapply in_mth; eauto.
+        eapply substmt_trans;
+          eauto.
+        rewrite Ha0 in H5;
+          inversion H5;
+          subst;
+          crush.
+
+      * right.
+        repeat destruct_exists_loo;
+          andDestruct.
+        exists χ, ϕ0, ψ, α, m, β, s2;
+          repeat split;
+          auto.
+        inversion Hb; subst.
+        eapply in_mth; eauto.
+        eapply substmt_trans;
+          eauto.
+        rewrite Ha1 in H5;
+          inversion H5;
+          subst;
+          crush.
+
+    + simpl in *.
+      destruct (IHHred χ1 χ2 ϕ1 ϕ ψ1 (ϕ'::ψ2)) as [Ha|Ha];
+        auto.
+      * left; auto.
+        repeat destruct_exists_loo;
+          andDestruct.
+        exists α0, m, β, s;
+          repeat split;
+          auto.
+        inversion Hb0;
+          subst.
+        eapply in_mth; eauto.
+        eapply substmt_trans;
+          eauto.
+        rewrite Ha0 in H5;
+          inversion H5;
+          subst;
+          crush.
+
+      * right.
+        repeat destruct_exists_loo;
+          andDestruct.
+        exists χ, ϕ0, ψ, α0, m, β, s;
+          repeat split;
+          auto.
+        inversion Hb; subst.
+        eapply in_mth; eauto.
+        eapply substmt_trans;
+          eauto.
+        rewrite Ha1 in H1;
+          inversion H1;
+          subst;
+          crush.
+        crush.
+
+    + simpl in *.
+      destruct (IHHred χ1 χ2 ϕ1 ϕ ψ1 (ϕ'::ψ2)) as [Ha|Ha];
+        auto.
+      * left; auto.
+        repeat destruct_exists_loo;
+          andDestruct.
+        exists α0, m, β, s;
+          repeat split;
+          auto.
+        inversion Hb0;
+          subst.
+        eapply in_mth; eauto.
+        eapply substmt_trans;
+          eauto.
+        rewrite Ha1 in H1;
+          inversion H1;
+          subst;
+          crush.
+        crush.
+
+      * right.
+        repeat destruct_exists_loo;
+          andDestruct.
+        exists χ, ϕ0, ψ, α0, m, β, s;
+          repeat split;
+          auto.
+        inversion Hb; subst.
+        eapply in_mth; eauto.
+        eapply substmt_trans;
+          eauto.
+        rewrite Ha1 in H1;
+          inversion H1;
+          subst;
+          crush.
+        crush.
+
+Qed.*)
+
+Lemma bottom_frame_remains_in_stack_reduction :
+  forall M σ1 σ2, M ∙ σ1 ⤳ σ2 ->
+             forall χ1 ϕ1 ψ1,
+               σ1 = (χ1, ψ1 ++ ϕ1 :: nil) ->
+               exists ψ ϕ, (snd σ2) = (ψ ++ ϕ :: nil) /\
+                      vMap ϕ this = vMap ϕ1 this.
+Proof.
+  intros M σ1 σ2 Hred;
+    induction Hred;
+    intros;
+    subst;
+    simpl in *;
+    repeat simpl_crush;
+    simpl;
+    try solve [repeat match goal with
+                      | [H : ?ϕ1 :: ?ψ1 = ?ψ2 ++ ?ϕ2 :: nil |- _] =>
+                        let ϕ := fresh "ϕ" in
+                        let ψ := fresh "ψ" in
+                        destruct ψ2 as [|ϕ ψ]; simpl in H; inversion H; subst
+                      end;
+               match goal with
+               | [|- exists ψ ϕ, ?ϕ' :: nil = ψ ++ ϕ :: nil /\ _] =>
+                 exists nil, ϕ'
+               | [|- exists ψ ϕ, ?ϕ'' :: ?ψ' ++ ?ϕ' :: nil = ψ ++ ϕ :: nil /\ _] =>
+                 exists (ϕ''::ψ'), ϕ'
+               | [|- exists ψ ϕ, ?ϕ'' :: ?ϕ' :: nil = ψ ++ ϕ :: nil /\ _] =>
+                 exists (ϕ'' :: nil), ϕ'
+               | [|- exists ψ ϕ, ?ϕ'' :: ?ϕ' :: ?ψ' ++ ?ϕ''' :: nil = ψ ++ ϕ :: nil /\ _] =>
+                 exists (ϕ'' :: ϕ' :: ψ'), ϕ'''
+               | [|- exists ψ ϕ, ?ϕ'' :: ?ϕ' :: ?ψ' = ψ ++ ϕ :: nil /\ _] =>
+                 exists (ϕ''::ψ'), ϕ'
+               end;
+               split;
+               auto;
+               simpl; repeat map_rewrite].
+Qed.
+
+Lemma bottom_frame_remains_in_stack_reductions :
+  forall M σ1 σ2, reductions M σ1 σ2 ->
+             forall χ1 ϕ1 ψ1,
+               σ1 = (χ1, ψ1 ++ ϕ1 :: nil) ->
+               exists ψ ϕ, (snd σ2) = (ψ ++ ϕ :: nil) /\
+                      vMap ϕ this = vMap ϕ1 this.
+Proof.
+  intros M σ1 σ2 Hred;
+    induction Hred;
+    intros;
+    subst.
+
+  - eapply bottom_frame_remains_in_stack_reduction; eauto.
+
+  - destruct (IHHred χ1 ϕ1 ψ1); auto;
+      destruct_exists_loo;
+      andDestruct;
+        subst.
+
+    destruct σ2 as [χ ψ];
+      simpl in *;
+      subst.
+    rewrite <- Hb.
+    apply (bottom_frame_remains_in_stack_reduction M (χ, x++ϕ :: nil)) with (χ1:=χ)(ψ1:=x);
+      auto.
+Qed.
+
+Lemma different_this_implies_larger_stack_reductions :
+  forall M σ1 σ2, reductions M σ1 σ2 ->
+             σ_wf σ1 ->
+             forall χ1 ϕ1,
+               σ1 = (χ1, ϕ1 :: nil) ->
+               forall v1 v2, ⌊ this ⌋ σ1 ≜ v1 ->
+                        ⌊ this ⌋ σ2 ≜ v2 ->
+                        (length (snd σ1) < length (snd σ2)) \/
+                        (v1 = v2 /\ length (snd σ1) = length (snd σ2)).
+Proof.
+  intros.
+  destruct (bottom_frame_remains_in_stack_reductions M σ1 σ2 H χ1 ϕ1 nil)
+    as [ψ];
+    auto;
+    destruct_exists_loo;
+    andDestruct.
+  destruct σ2 as [χ2 ψ2];
+    simpl in *;
+    subst;
+    simpl in *.
+
+  destruct ψ as [|ϕ' ψ'];
+    simpl in *.
+  - match goal with
+    | [Ha : ⌊ ?x ⌋ ?σ1 ≜ _,
+            Hb : ⌊ ?x ⌋ ?σ2 ≜ _ |- _] =>
+      inversion Ha;
+        inversion Hb;
+        subst
+    end;
+      simpl in *;
+      repeat simpl_crush.
+    match goal with
+    | [ Ha : vMap ?ϕ1 ?x = vMap ?ϕ2 ?x,
+             Hb : vMap ?ϕ1 ?x = Some _,
+                  Hc : vMap ?ϕ2 ?x = Some _ |- _] =>
+      rewrite Ha in Hb;
+        rewrite Hb in Hc
+    end;
+      crush.
+
+  - simpl;
+      rewrite app_length;
+      crush.
+Qed.
+
+Lemma reduction_implies_non_empty_stack_1 :
+  forall M σ1 σ2, M ∙ σ1 ⤳ σ2 ->
+             exists χ1 ϕ1 ψ1, σ1 = (χ1, ϕ1 :: ψ1).
+Proof.
+  intros M σ1 σ2 Hred;
+    induction Hred;
+    intros;
+    eauto.
+Qed.
+
+Lemma reduction_implies_non_empty_stack_2 :
+  forall M σ1 σ2, M ∙ σ1 ⤳ σ2 ->
+             exists χ2 ϕ2 ψ2, σ2 = (χ2, ϕ2 :: ψ2).
+Proof.
+  intros M σ1 σ2 Hred;
+    induction Hred;
+    intros;
+    eauto.
+Qed.
+
+Lemma reduction_preserves_heap_locations :
+  forall M σ1 σ2, M ∙ σ1 ⤳ σ2 ->
+             forall α (o : obj), mapp σ1 α = Some o ->
+                            exists o', mapp σ2 α = Some o'.
+Proof.
+  intros M σ1 σ2 Hred;
+    induction Hred;
+    intros;
+    eauto;
+    subst;
+    try solve [repeat eexists;
+               crush;
+               eauto];
+    try solve [destruct (eq_dec α α0);
+               subst;
+               repeat map_rewrite;
+               eauto].
+Qed.
+
+Lemma reductions_preserves_heap_locations_classes :
+  forall M σ1 σ2, reductions M σ1 σ2 ->
+             forall α (o : obj), mapp σ1 α = Some o ->
+                            exists o', mapp σ2 α = Some o' /\
+                                  cname o' = cname o.
+Proof.
+  intros M σ1 σ2 Hred;
+    induction Hred;
+    intros.
+
+  - eapply reduction_preserves_addr_classes;
+      eauto.
+
+  - specialize (IHHred α o);
+      auto_specialize;
+      destruct_exists_loo;
+      andDestruct.
+    apply reduction_preserves_addr_classes
+            with (α:=α)(o1:=o0) in H;
+      eauto;
+      repeat destruct_exists_loo;
+      andDestruct.
+    eexists; split; eauto; crush.
+Qed.
+
+Lemma reduction_preserves_fields :
+  forall M σ1 σ2, M ∙ σ1 ⤳ σ2 ->
+             forall α o f v, mapp σ1 α = Some o ->
+                        flds o f = Some v ->
+                        exists o' v', mapp σ2 α = Some o' /\
+                                 flds o' f = Some v'.
+Proof.
+  intros M σ1 σ2 Hred;
+    induction Hred;
+    intros;
+    eauto;
+    try solve [repeat eexists; crush; eauto].
+
+  - destruct (eq_dec α α0);
+      subst;
+      destruct (eq_dec f0 f);
+      subst;
+      repeat map_rewrite;
+      eauto.
+    + repeat eexists;
+        eauto;
+        unfold flds;
+        eq_auto.
+    + match goal with
+      | [|- exists o' _, Some ?o = Some o' /\ _ ] =>
+        exists o
+      end.
+      exists v0;
+        split;
+        eauto;
+        unfold flds;
+        eq_auto.
+      match goal with
+      | [Ha : ?m ?a = _,
+              Hb : ?m ?a = _ |- _] =>
+        rewrite Ha in Hb;
+          inversion Hb;
+          subst
+      end.
+      destruct o0;
+        auto.
+
+  - subst.
+    destruct (eq_dec α α0);
+      subst;
+      repeat map_rewrite;
+      eauto.
+    eapply fresh_heap_some_contradiction; eauto.
+Qed.
+
+Lemma reductions_preserves_fields :
+  forall M σ1 σ2, reductions M σ1 σ2 ->
+             forall α o f v, mapp σ1 α = Some o ->
+                        flds o f = Some v ->
+                        exists o' v', mapp σ2 α = Some o' /\
+                                 flds o' f = Some v'.
+Proof.
+  intros M σ1 σ2 Hred;
+    induction Hred;
+    intros.
+
+  - eapply reduction_preserves_fields; eauto.
+
+  - specialize (IHHred α o f v);
+      repeat auto_specialize;
+      repeat destruct_exists_loo;
+      andDestruct.
+    eapply reduction_preserves_fields;
+      eauto.
+Qed.
+
+Lemma reductions_field_change :
+  forall M σ1 σ2, reductions M σ1 σ2 ->
+             forall χ1 ϕ1 ψ1 χ2 ϕ2 ψ2,
+               σ1 = (χ1, ϕ1 :: ψ1) ->
+               σ2 = (χ2, ϕ2 :: ψ2) ->
+               forall α o1 o2 f v1 v2,
+                 mapp σ1 α = Some o1 ->
+                 mapp σ2 α = Some o2 ->
+                 flds o1 f = Some v1 ->
+                 flds o2 f = Some v2 ->
+                 v1 <> v2 ->
+                 exists χ ϕ ψ, (reductions M σ1 (χ, ϕ :: ψ) \/ σ1 = (χ, ϕ :: ψ)) /\
+                          exists  x y s C, contn ϕ = c_stmt ((x ◌ f) ≔ (r_ y) ;; s) /\
+                                      ⌊ x ⌋ (χ, ϕ :: ψ) ≜ (v_addr α) /\
+                                      classOf this (χ, ϕ :: ψ) C /\
+                                      classOf x (χ, ϕ :: ψ) C /\
+                                      ⌊ y ⌋ (χ, ϕ :: ψ) ≜ v2.
+Proof.
+  intros.
+  destruct (reductions_prop_change M σ1 σ2)
+    with (P:= fun σ : config => forall o, mapp σ α = Some o -> flds o f = Some v2);
+    auto.
+  - intros Hcontra;
+      specialize (Hcontra o1);
+      auto_specialize;
+      crush.
+
+  - intros;
+      crush.
+
+  - destruct_exists_loo;
+      andDestruct.
+    destruct x as [χa ψa];
+      destruct σ as [χb ψb].
+    edestruct (reduction_implies_non_empty_stack_1 M (χa, ψa));
+      eauto.
+    edestruct (reduction_implies_non_empty_stack_2 M (χa, ψa) (χb, ψb));
+      eauto;
+      repeat destruct_exists_loo;
+      repeat simpl_crush.
+    exists x, ϕ0, ψ0;
+      split;
+      auto.
+
+    match goal with
+    | [ Ha : reductions _ _ _ \/ _,
+             Hb : reductions _ _ _ \/ _ |- _] =>
+      destruct Ha, Hb
+    end.
+    
+    + destruct (reductions_preserves_fields M (χ1, ϕ1 :: ψ1) (x, ϕ0 :: ψ0))
+        with (α:=α)(o:=o1)(f:=f)(v:=v1);
+        eauto with loo_db;
+        destruct_exists_loo;
+        andDestruct.
+      destruct (reduction_preserves_fields M (x, ϕ0 :: ψ0) (x0, ϕ :: ψ))
+        with (α:=α)(o:=x1)(f:=f)(v:=v);
+        eauto with loo_db;
+        destruct_exists_loo;
+        andDestruct.
+      eapply (reduction_field_change M (x, ϕ0 :: ψ0) (x0, ϕ :: ψ))
+        with (χ1:=x)(ψ1:=ψ0)(χ2:=x0);
+        eauto.
+      intros Hcontra;
+        subst.
+      contradiction Ha0;
+        intros.
+      repeat map_rewrite.
+      rewrite Ha2 in H7;
+        inversion H7;
+        subst;
+        auto.
+
+    + repeat simpl_crush.
+      destruct (reductions_preserves_fields M (χ1, ϕ1 :: ψ1) (x, ϕ0 :: ψ0))
+        with (α:=α)(o:=o1)(f:=f)(v:=v1);
+        eauto with loo_db;
+        destruct_exists_loo;
+        andDestruct.
+      destruct (reduction_preserves_fields M (x, ϕ0 :: ψ0) (x0, ϕ :: ψ))
+        with (α:=α)(o:=x1)(f:=f)(v:=v);
+        eauto with loo_db;
+        destruct_exists_loo;
+        andDestruct.
+      eapply (reduction_field_change M (x, ϕ0 :: ψ0) (x0, ϕ :: ψ))
+        with (χ1:=x)(ψ1:=ψ0)(χ2:=x0);
+        eauto.
+      intros Hcontra;
+        subst.
+      contradiction Ha0;
+        intros.
+      repeat map_rewrite.
+      rewrite Ha2 in H1;
+        inversion H1;
+        subst;
+        auto.
+
+    + repeat simpl_crush.
+      destruct (reduction_preserves_fields M (x, ϕ0 :: ψ0) (x0, ϕ :: ψ))
+        with (α:=α)(o:=o1)(f:=f)(v:=v1);
+        eauto with loo_db;
+        destruct_exists_loo;
+        andDestruct.
+      destruct (reductions_preserves_fields M (x0, ϕ :: ψ) (χ2, ϕ2 :: ψ2))
+        with (α:=α)(o:=x1)(f:=f)(v:=v);
+        eauto with loo_db;
+        destruct_exists_loo;
+        andDestruct.
+      eapply (reduction_field_change M (x, ϕ0 :: ψ0) (x0, ϕ :: ψ))
+        with (χ1:=x)(ψ1:=ψ0)(χ2:=x0);
+        eauto.
+
+    + repeat simpl_crush.
+      eapply reduction_field_change; eauto.
+
+Qed.
+
+Lemma frame_arising_from_single_frame_is_method_call_reductions :
+  forall M σ1 σ2, reductions M σ1 σ2 ->
+             forall χ1 ϕ1,
+               σ1 = (χ1, ϕ1 :: nil) ->
+               mapp σ1 this <> mapp σ2 this ->
+               forall χ2 ϕ2 ψ2, σ2 = (χ2, ϕ2 :: ψ2) ->
+                           (exists α m β s, method_is_called σ1 α m β /\
+                                       contn ϕ2 = c_stmt s /\
+                                       stmt_in_method M χ1 α m s) \/
+                           (exists χ ϕ ψ α m β s, reductions M σ1 (χ, ϕ :: ψ) /\
+                                             method_is_called (χ, ϕ :: ψ) α m β /\
+                                             contn ϕ2 = c_stmt s /\
+                                             stmt_in_method M χ α m s).
+Proof.
+  intros.
+(*  destruct (arising_frame_is_method_call_reductions M σ1 σ2)
+    with
+      (χ1:=χ1)(χ2:=χ2)(ϕ1:=ϕ1)(ϕ2:=ϕ2)(ψ1:=@nil frame)(ψ2:=ψ2);
+    simpl;
+    auto.
+
+  let ψ := fresh "ψ" in
+  let ϕ := fresh "ϕ" in
+  edestruct (bottom_frame_remains_in_stack_reductions M σ1 σ2)
+    with
+      (ψ1:=@nil frame) as [ψ Htmp];
+    eauto;
+    destruct Htmp as [ϕ];
+    andDestruct;
+    subst;
+    simpl in *.
+
+  let ϕ' := fresh "ϕ" in
+  let ψ' := fresh "ψ" in
+  destruct ψ as [|ϕ' ψ'];
+    simpl in *;
+    simpl_crush;
+    repeat map_rewrite;
+    try rewrite app_length; crush.*)
+Admitted.
+
+Lemma reductions_field_change_not_this :
+  forall M σ1 σ2, reductions M σ1 σ2 ->
+             forall χ1 ϕ1 ψ1 χ2 ϕ2 ψ2,
+               σ1 = (χ1, ϕ1 :: ψ1) ->
+               σ2 = (χ2, ϕ2 :: ψ2) ->
+               forall α o1 o2 f v1 v2,
+                 mapp σ1 α = Some o1 ->
+                 mapp σ2 α = Some o2 ->
+                 flds o1 f = Some v1 ->
+                 flds o2 f = Some v2 ->
+                 v1 <> v2 ->
+                 (forall C, classOf this σ1 C ->
+                       cname o1 <> C) ->
+                 exists χ ϕ ψ x y s C, reductions M σ1 (χ, ϕ :: ψ) /\
+                                  contn ϕ = c_stmt ((x ◌ f) ≔ (r_ y) ;; s) /\
+                                  ⌊ x ⌋ (χ, ϕ :: ψ) ≜ (v_addr α) /\
+                                  classOf this (χ, ϕ :: ψ) C /\
+                                  classOf x (χ, ϕ :: ψ) C /\
+                                  ⌊ y ⌋ (χ, ϕ :: ψ) ≜ v2.
+Proof.
+  intros.
+  let χ := fresh "χ" in
+  edestruct (reductions_field_change M σ1 σ2)
+    as [χ];
+    eauto;
+    repeat destruct_exists_loo;
+    andDestruct;
+    repeat destruct_exists_loo;
+    andDestruct.
+  exists χ, ϕ, ψ, x, x0, s, C;
+    repeat split;
+    auto.
+  destruct Ha;
+    subst;
+    auto;
+    simpl_crush.
+  specialize (H7 C);
+    auto_specialize.
+  repeat map_rewrite.
+  inversion Ha3;
+    subst;
+    simpl in *.
+  interpretation_rewrite.
+  inversion H0;
+    subst.
+  rewrite H2 in H8;
+    inversion H8;
+    subst;
+    crush.
+Qed.
+
+Definition is_internal (M1 M2 : mdl)(σ : config) :=
+  (exists α o CDef, mapp σ this = Some (v_addr α) /\
+               mapp σ α = Some o /\
+               M1 (cname o) = Some CDef).
+
+Definition is_external (M1 M2 : mdl)(σ : config) :=
+  (exists α o, mapp σ this = Some (v_addr α) /\
+          mapp σ α = Some o /\
+          M1 (cname o) = None).
+
+Lemma frame_arising_from_single_frame_external_internal_is_method_call_reductions :
+  forall M σ1 σ2, reductions M σ1 σ2 ->
+             forall χ1 ϕ1,
+               σ1 = (χ1, ϕ1 :: nil) ->
+               forall M1 M2,
+                 M1 ⋄ M2 ≜ M ->
+                 is_external M1 M2 σ1 ->
+                 is_internal M1 M2 σ2 ->
+                 forall χ2 ϕ2 ψ2, σ2 = (χ2, ϕ2 :: ψ2) ->
+                             (exists α m β s, method_is_called σ1 α m β /\
+                                         contn ϕ2 = c_stmt s /\
+                                         stmt_in_method M χ1 α m s) \/
+                             (exists χ ϕ ψ α m β s, reductions M σ1 (χ, ϕ :: ψ) /\
+                                               method_is_called (χ, ϕ :: ψ) α m β /\
+                                               contn ϕ2 = c_stmt s /\
+                                               stmt_in_method M χ α m s).
+Proof.
+  intros.
+  eapply frame_arising_from_single_frame_is_method_call_reductions;
+    eauto.
+  unfold is_external, is_internal in *;
+    repeat destruct_exists_loo;
+    andDestruct;
+    subst;
+    repeat map_rewrite.
+  intros Hcontra;
+    rewrite Hcontra in *.
+  rewrite Ha in Ha1;
+    inversion Ha1;
+    subst.
+
+  let o' := fresh "o" in
+  destruct (reductions_preserves_heap_locations_classes M (χ1, ϕ1::nil)(χ2, ϕ2 :: ψ2))
+    with (α:=α0)(o:=o0) as [o'];
+    auto;
+    andDestruct.
+  repeat map_rewrite.
+  rewrite Ha0 in Ha3;
+    inversion Ha3;
+    subst.
+  rewrite Hb in *;
+    crush.
+Qed.
+
+Lemma is_external_implies_not_is_internal :
+  forall M1 M2 σ, is_external M1 M2 σ ->
+             ~ is_internal M1 M2 σ.
+Proof.
+  intros;
+    unfold is_internal, is_external in *;
+    intro Hcontra;
+    repeat destruct_exists_loo;
+    andDestruct;
+    crush.
+Qed.
+
+Lemma is_internal_implies_not_is_external :
+  forall M1 M2 σ, is_internal M1 M2 σ ->
+             ~ is_external M1 M2 σ.
+Proof.
+  intros;
+    intro Hcontra;
+    unfold is_internal, is_external in *;
+    repeat destruct_exists_loo;
+    andDestruct;
+    crush.
+Qed.
+
+Inductive stack_trace : mdl -> mdl -> config -> Prop :=
+| trace_initial : forall M1 M2 χ ϕ x s, is_external M1 M2 (χ, ϕ :: nil) ->
+                                   classOf this (χ, ϕ :: nil) ObjectName ->
+                                   contn ϕ = c_hole x s ->
+                                   stack_trace M1 M2 (χ, ϕ :: nil)
+| trace_internal : forall M1 M2 χ ϕ ψ x s C CDef m zs body,
+    stack_trace M1 M2 (χ, ψ) ->
+    contn ϕ = c_hole x s ->
+    classOf this (χ, ϕ :: ψ) C ->
+    M1 C = Some CDef ->
+    M2 C = None ->
+    c_meths CDef m = Some (zs, body) ->
+    substmt s body ->
+    stack_trace M1 M2 (χ, ϕ :: ψ)
+| trace_external : forall M1 M2 χ ϕ ϕ' ψ x s C CDef m zs body,
+    stack_trace M1 M2 (χ, ψ) ->
+    contn ϕ = c_hole x s ->
+    classOf this (χ, ϕ :: ϕ' :: ψ) C ->
+    M1 C = None ->
+    M2 C = Some CDef ->
+    c_meths CDef m = Some (zs, body) ->
+    substmt s body ->
+    stack_trace M1 M2 (χ, ϕ :: ϕ' :: ψ).
+
+Inductive valid_stack_trace : mdl -> mdl -> config -> Prop :=
+| int_head : forall M1 M2 χ ϕ ψ s C CDef m zs body,
+    stack_trace M1 M2 (χ, ψ) ->
+    contn ϕ = c_stmt s ->
+    classOf this (χ, ϕ :: ψ) C ->
+    M1 C = Some CDef ->
+    M2 C = None ->
+    c_meths CDef m = Some (zs, body) ->
+    substmt s body ->
+    valid_stack_trace M1 M2 (χ, ϕ :: ψ)
+| ext_head : forall M1 M2 χ ϕ ψ s C CDef m zs body,
+    stack_trace M1 M2 (χ, ψ) ->
+    contn ϕ = c_stmt s ->
+    classOf this (χ, ϕ :: ψ) C ->
+    M1 C = None ->
+    M2 C = Some CDef ->
+    c_meths CDef m = Some (zs, body) ->
+    substmt s body ->
+    valid_stack_trace M1 M2 (χ, ϕ :: ψ).
+
+Hint Constructors valid_stack_trace stack_trace : loo_db.
+
+Lemma valid_program_trace_reduction :
+  forall M σ1 σ2, M ∙ σ1 ⤳ σ2 ->
+             forall M1 M2,
+               M_wf M1 ->
+               M1 ⋄ M2 ≜ M ->
+               valid_stack_trace M1 M2 σ1 ->
+               valid_stack_trace M1 M2 σ2.
+Proof.
+  intros M σ1 σ2 Hred;
+    induction Hred;
+    intros;
+    subst.
+
+  - admit.
+
+  - match goal with
+    | [H : valid_stack_trace _ _ _ |- _] =>
+      inversion H;
+        subst
+    end;
+      match goal with
+      | [Ha : ?M1 ?C = Some ?CDef,
+              Hb : ?M2 ?C = None,
+                   Hc : c_meths ?CDef ?m = Some (?zs, ?body),
+                        Hd : contn ?ϕ = c_stmt (_ ;; ?s)
+         |- valid_stack_trace ?M1 ?M2 (_, _)] =>
+        eapply (int_head M1 M2 χ) with (C:=C)(CDef:=CDef)(m:=m)(s:=s)(zs:=zs)(body:=body);
+          eauto
+      | [Ha : ?M1 ?C = None,
+              Hb : ?M2 ?C = Some ?CDef,
+                   Hc : c_meths ?CDef ?m = Some (?zs, ?body),
+                        Hd : contn ?ϕ = c_stmt (_ ;; ?s)
+         |- valid_stack_trace ?M1 ?M2 (_, _)] =>
+        eapply (ext_head M1 M2 χ) with (C:=C)(CDef:=CDef)(m:=m)(s:=s)(zs:=zs)(body:=body);
+          eauto
+      end;
+      try solve [match goal with
+                 | [Hcls : classOf _ _ _ |- _] =>
+                   inversion Hcls;
+                   subst;
+                   simpl in *
+                 end;
+                 eapply cls_of; simpl; eauto;
+                 match goal with
+                 | [Hint : interpret_x _ _ _ |- _] =>
+                   inversion Hint;
+                   subst;
+                   simpl in *;
+                   repeat simpl_crush
+                 end;
+                 eapply int_x; simpl; eauto; simpl;
+                 repeat map_rewrite;
+                 auto];
+      try solve [ match goal with
+                  | [Ha : contn ?ϕ = _,
+                          Hb : contn ?ϕ = _,
+                               Hsub : substmt _ _ |- _] =>
+                    rewrite Ha in Hb;
+                    inversion Hb;
+                    subst
+                  end;
+                  apply substmt_trans with (s2:= (x ≔′ e) ;; s);
+                  crush].
+
+  - match goal with
+    | [H : valid_stack_trace _ _ _ |- _] =>
+      inversion H;
+        subst
+    end;
+      match goal with
+      | [Ha : ?M1 ?C' = Some ?CDef,
+              Hb : ?M2 ?C' = None,
+                   Hc : c_meths ?CDef ?m = Some (?zs, ?body),
+                        Hd : contn ?ϕ = c_stmt (_ ;; ?s)
+         |- valid_stack_trace ?M1 ?M2 (_, _)] =>
+        eapply (int_head M1 M2 χ) with (C:=C')(CDef:=CDef)(m:=m)(s:=s)(zs:=zs)(body:=body);
+          eauto
+      | [Ha : ?M1 ?C' = None,
+              Hb : ?M2 ?C' = Some ?CDef,
+                   Hc : c_meths ?CDef ?m = Some (?zs, ?body),
+                        Hd : contn ?ϕ = c_stmt (_ ;; ?s)
+         |- valid_stack_trace ?M1 ?M2 (_, _)] =>
+        eapply (ext_head M1 M2 χ) with (C:=C')(CDef:=CDef)(m:=m)(s:=s)(zs:=zs)(body:=body);
+          eauto
+      end;
+    
+      try solve [match goal with
+                 | [Hcls : classOf _ _ _ |- _] =>
+                   inversion Hcls;
+                   subst;
+                   simpl in *
+                 end;
+                 eapply cls_of; simpl; eauto;
+                 match goal with
+                 | [Hint : interpret_x _ _ _ |- _] =>
+                   inversion Hint;
+                   subst;
+                   simpl in *;
+                   repeat simpl_crush
+                 end;
+                 eapply int_x; simpl; eauto; simpl;
+                 repeat map_rewrite;
+                 auto];
+      try solve [ match goal with
+                  | [Ha : contn ?ϕ = _,
+                          Hb : contn ?ϕ = _,
+                               Hsub : substmt _ _ |- _] =>
+                    rewrite Ha in Hb;
+                    inversion Hb;
+                    subst
+                  end;
+                  apply substmt_trans with (s2:= ((r_ x) ≔ (y ◌ f)) ;; s);
+                  crush].
+
+  - (*match goal with
+    | [H : valid_stack_trace _ _ _ |- _] =>
+      inversion H;
+        subst
+    end;
+      match goal with
+      | [Ha : ?Ma ?C' = Some ?CDef',
+              Hb : ?Mb ?C' = None,
+                   Hc : c_meths ?CDef' ?m' = Some (?zs', ?body'),
+                        Hd : contn ?ϕ' = c_stmt (_ ;; ?s')
+         |- valid_stack_trace ?Ma ?Mb (?χ', _)] =>
+        eapply (int_head Ma Mb χ') with (C:=C')(CDef:=CDef')(m:=m')(s:=s')(zs:=zs')(body:=body');
+          eauto
+      | [Ha : ?Ma ?C' = None,
+              Hb : ?Mb ?C' = Some ?CDef',
+                   Hc : c_meths ?CDef' ?m' = Some (?zs', ?body'),
+                        Hd : contn ?ϕ' = c_stmt (_ ;; ?s')
+         |- valid_stack_trace ?Ma ?Mb (?χ', _)] =>
+        eapply (ext_head Ma Mb χ') with (C:=C')(CDef:=CDef')(m:=m')(s:=s')(zs:=zs')(body:=body');
+          eauto
+      end.*)
+    admit.
+
+  - admit.
+
+  - 
+
+
+Admitted.
+
+Lemma reduction_internal_external :
+  forall M σ1 σ2, M ∙ σ1 ⤳ σ2 ->
+             M_wf M ->
+             forall χ1 ϕ1 ψ1 χ2 ϕ2 ψ2, σ1 = (χ1, ϕ1 :: ψ1) ->
+                                  σ2 = (χ2, ϕ2 :: ψ2) ->
+                                  forall M1 M2, M1 ⋄ M2 ≜ M ->
+                                           is_external M1 M2 σ1 ->
+                                           (is_external M1 M2 σ2 \/
+                                            (is_internal M1 M2 σ2 /\
+                                             exists C CDef m zs s s', classOf this σ2 C /\
+                                                                 M1 C = Some CDef /\
+                                                                 c_meths CDef m = Some (zs, s) /\
+                                                                 contn ϕ2 = c_stmt s' /\
+                                                                 substmt s' s)).
+Proof.
+  intros M σ1 σ2 Hred;
+    induction Hred;
+    intros;
+    repeat simpl_crush;
+    try solve [left;
+               unfold is_external;
+               repeat (map_rewrite; simpl)];
+    try solve [crush; eauto].
+
+  - (*destruct (partial_map_dec (cname o) M1);
+      [repeat destruct_exists_loo; right; left|left].
+    + split; [unfold is_internal|].
+      * repeat map_rewrite;
+          simpl;
+          repeat eexists; eauto.
+      * exists (cname o), C, m, zs, s, s;
+          repeat split;
+          auto.
+        ** eapply cls_of; eauto.
+           eapply int_x; simpl; eauto.
+        ** inversion H12;
+             subst.
+           repeat map_rewrite.
+           unfold extend in H4;
+             rewrite H0 in H4;
+             inversion H4;
+             subst;
+             auto.
+        ** apply sub_refl.
+
+    + unfold is_external; eauto;
+        repeat map_rewrite;
+        simpl.
+      repeat eexists; eauto.
+
+  - subst;
+      repeat simpl_crush.
+    left;
+      unfold is_external.
+    exists α, {| cname := cname o; flds := update f v (flds o); meths := meths o |}; simpl;
+      repeat split;
+      repeat map_rewrite;
+      auto.
+    
+    
+    
+    repeat (map_rewrite; simpl);
+      split;
+      auto.
+      simpl.
+      repeat (map_rewrite; simpl).
+      subst.*)
+
+    
+      
+Admitted.
 
 Module SafeExample.
 
@@ -17,7 +1395,6 @@ Module SafeExample.
 ∀s.[s : Safe ∧ s.treasure <> null ∧ will(s.treasure = null) 
         ⟶ ∃o.[external(o) ∧ (o access s.secret)]]
  *)
-  
 
   (** Safe Definition *)
 
@@ -31,21 +1408,64 @@ Module SafeExample.
 
   Definition scr := bnd 0.
 
-  Definition takeBody := s_stmts (s_if (e_eq scr (e_acc_f this secret) )).
+  Definition x := bnd 1.
 
-  Definition SafeDef := clazz Safe
-                              (treasure :: secret :: nil)
-                              (update
-                                 take (nil, takeBody)
-                                 empty)
-                              empty.
+  Definition y := bnd 2.
+
+  Definition takeBody := ((r_ x) ≔ (r_exp (e_val (v_null))) ;;
+                         (s_if ((e_var scr) ⩵ (e_acc_f (e_var this) secret))
+                               ((r_ y) ≔ (this ◌ secret) ;; ((this ◌ secret) ≔ (r_ x)) ;; (s_rtrn y))
+                               (s_rtrn x)) ;;
+                         (s_rtrn x)).
+
+  Definition SafeDef1 := clazz Safe
+                               (treasure :: secret :: nil)
+                               (update
+                                  take (scr :: nil, takeBody)
+                                  empty)
+                               empty.
 
   (** MyModule Definition *)
 
-  Definition MyModule := (update
-                            Boundary BoundaryDef
-                            (update
-                               Inside InsideDef
-                               empty)).
+  Definition MyModule1 := (update
+                             Safe SafeDef1
+                             empty).    
+
+  Definition HolisticSpec := (∀x∙ (∀x∙(((a_class (a♢1) Safe)
+                                        ∧
+                                        ((ex_acc_f (e♢1) secret) ⩶ (e♢0))
+                                        ∧
+                                        ((ex_acc_f (e♢1) treasure) ⩶̸ (ex_null))
+                                        ∧
+                                        (a_will (((ex_acc_f (e♢1) treasure) ⩶ (ex_null)))))
+                                         ⟶
+                                         (∃x∙ (((a♢0) external)
+                                               ∧
+                                               ((a♢0) access (a♢1))))
+                             ))).
+
+  Theorem safe_example :
+    MyModule1 ⊨m HolisticSpec.
+  Proof.
+    unfold mdl_sat;
+      intros;
+      destruct_exists_loo.
+    unfold HolisticSpec;
+      a_intros.
+    a_prop.
+    inversion H5;
+      subst.
+
+    let χ := fresh "χ" in
+    let ψ := fresh "ψ" in
+    destruct σ' as [χ ψ].
+
+    assert (exists ϕ' ψ', ψ0 = ϕ' :: ψ');
+      [admit|repeat destruct_exists_loo; subst].
+    (*destruct (reductions_field_change M (χ, ϕ :: nil) (χ0, ϕ0 :: ψ1))
+      with (χ1:=χ)(ϕ1:=ϕ)(ψ2:=ψ1)(χ2:=χ0)(ϕ2:=ϕ0)(f:=treasure).*)
+              
+  Admitted.
 
 End SafeExample.
+
