Coq/DAO.v
@@ -1,0 +1,57 @@
+Require Import common.
+Require Import loo_def.
+Require Import loo_properties.
+Require Import loo_reduction_properties.
+Require Import decoupled_classical_properties.
+Require Import decoupling.
+Require Import function_operations.
+Require Import List.
+Require Import CpdtTactics.
+Require Import Coq.Logic.FunctionalExtensionality.
+
+Print reduction.
+
+Module SafeExample.
+
+(**
+∀s.[s : Safe ∧ s.treasure <> null ∧ will(s.treasure = null) 
+        ⟶ ∃o.[external(o) ∧ (o access s.secret)]]
+ *)
+  
+
+  (** DAO Definition *)
+
+  Definition Safe := classID 1.
+
+  Definition treasure := fieldID 0.
+
+  Definition secret := fieldID 1.
+
+  Definition take := methID 0.
+
+  Definition scr := bnd 0.
+
+  Definition x := bnd 1.
+
+  Definition y := bnd 2.
+
+  Definition takeBody := (x ⩦ (e_null);
+                         (s_if ((e_var scr) ⩵ (e_acc_f (e_var this) secret))
+                               ((r_ y) ⩦′ (this ◌ secret) ; ((this ◌ secret) ⩦′ (r_ x)) ; (s_rtrn y))
+                               (s_rtrn x)) ;
+                         (s_rtrn x)).
+
+  Definition SafeDef := clazz Safe
+                              (treasure :: secret :: nil)
+                              (update
+                                 take (scr :: nil, takeBody)
+                                 empty)
+                              empty.
+
+  (** MyModule Definition *)
+
+  Definition MyModule := (update
+                            Safe SafeDef
+                            empty).
+
+End SafeExample.
